added and proved query for casual case

segmentTreeProof.dfy
@@ -68,8 +68,30 @@ module Monoid {
         constructor() {
         }
     }
-
+    trait Transform<U(!new), T(!new)> {
+        var monoid: AbstractMonoid<T>
+        function method identity(): U
+        function method apply(elem: U, res: T): T
+        function method compose(elem1: U, elem2: U): U
+        predicate hasIdentity() {
+            forall x: T :: apply(identity(), x) == x
+        } 
+        predicate isComposeAssociative() {
+            forall x: U, y: U, z: T :: apply(compose(x, y), z) == apply(x, apply(y, z))
+        }
+        predicate isDustrubutive() 
+            reads this
+        {
+            forall x: U, y: T, z: T :: apply(x, monoid.op(y, z)) == monoid.op(apply(x, y), apply(x, z))
+        }
+        predicate validTransform() 
+            reads this
+        {
+            isComposeAssociative() && isDustrubutive() && hasIdentity()
+        }
+    }
 }
+
 datatype SegmentTree<T> =
     Leaf(m: int, value: T)
     | Node(l: int, m: int, r: int, left: SegmentTree, right: SegmentTree, value: T)
@@ -98,21 +120,6 @@ predicate validTree(st: SegmentTree)
                 case Node(l2, m2, r2, _, _, _) =>
                     l2 == mm + 1 && r2 == rr
                 })
-    }
-}
-
-predicate validTreeValues<T(!new)>(tree: SegmentTree<T>, arr: array<T>, l: int, r: int, monoid: Monoid.AbstractMonoid<T>)
-    reads arr
-    requires 0 <= l <= r < arr.Length
-    requires validTree(tree)
-    requires boundaries(tree) == (l, r) 
-{
-    match tree {
-        case Leaf(l, val) => arr[l] == val
-        case Node(l, m, r, left, right, val) => 
-            validTreeValues(left, arr, l, m, monoid) && 
-            validTreeValues(right, arr, m + 1, r, monoid) &&
-            val == monoid.op(getValue(left), getValue(right))
     }
 }
 
@@ -148,6 +155,33 @@ function method mergeTrees<T>(left: SegmentTree<T>, right: SegmentTree<T>, merge
     Node(boundaries(left).0, boundaries(left).1, boundaries(right).1, left, right, merge(getValue(left), getValue(right)))
 }
 
+function maxInt(left: int, right: int): int 
+{
+    if left < right then right else left
+}
+
+
+function minInt(left: int, right: int): int 
+{
+    if left > right then right else left
+}
+
+predicate validTreeValues<T(!new)>(tree: SegmentTree<T>, arr: array<T>, monoid: Monoid.AbstractMonoid<T>)
+    reads arr
+    requires monoid.validMonoid()
+    requires 0 <= boundaries(tree).0 <= boundaries(tree).1 < arr.Length
+    requires validTree(tree)
+{
+    var (l, r) := boundaries(tree);
+    match tree {
+        case Leaf(l, val) => arr[l] == val
+        case Node(l, m, r, left, right, val) => 
+            validTreeValues(left, arr, monoid) && 
+            validTreeValues(right, arr, monoid) &&
+            val == straightQuery(arr, l, r, monoid)
+    }
+}
+
 function method buildTree<T(!new)>(arr: array<T>, l: int, r: int, monoid: Monoid.AbstractMonoid<T>): (res: SegmentTree<T>)
     reads arr
     requires 0 <= l <= r < arr.Length
@@ -155,7 +189,7 @@ function method buildTree<T(!new)>(arr: array<T>, l: int, r: int, monoid: Monoid
     ensures boundaries(res) == (l, r)
     ensures getValue(res) == straightQuery(arr, l, r, monoid)
     ensures validTree(res)
-    ensures validTreeValues(res, arr, l, r, monoid)
+    ensures validTreeValues(res, arr, monoid)
     decreases r - l
 {
     if l == r 
@@ -190,26 +224,201 @@ lemma associativeQuery<T(!new)>(elems: array<T>, l: int, m: int, r: int, monoid:
     assert straightQuery(elems, l, r, monoid) == monoid.op(straightQuery(elems, l, m, monoid), straightQuery(elems, m + 1, r, monoid));
 }
 
+    
+lemma validTreeValuesRange<T(!new)>(tree: SegmentTree<T>, arr: array<T>, monoid: Monoid.AbstractMonoid<T>)
+    requires 0 <= boundaries(tree).0  < arr.Length
+    requires 0 <= boundaries(tree).1  < arr.Length
+    requires monoid.validMonoid()
+    requires validTree(tree)
+    requires validTreeValues(tree, arr, monoid)
+    decreases boundaries(tree).1 - boundaries(tree).0
+    ensures straightQuery(arr, boundaries(tree).0, boundaries(tree).1, monoid) == getValue(tree)
+    ensures match tree {
+        case Leaf(x, val) => true
+        case Node(l, m, r, left, right, val) => monoid.op(getValue(left), getValue(right)) == val
+    }
+{
+    match tree {
+        case Leaf(x, val) => assert true;
+        case Node(l, m, r, left, right, val) => 
+            validTreeValuesRange(left, arr, monoid);
+            assert getValue(left) == straightQuery(arr, boundaries(left).0, boundaries(left).1, monoid);
+            validTreeValuesRange(right, arr, monoid);
+            assert getValue(right) == straightQuery(arr, boundaries(right).0, boundaries(right).1, monoid);
+            associativeQuery(arr, l, m, r, monoid);
+            assert monoid.op(getValue(left), getValue(right)) == val;
+    }
+}
+
+lemma equalArraysEqualQueries<T(!new)>(arr1: array<T>, arr2: array<T>, l: int, r: int, monoid: Monoid.AbstractMonoid<T>) 
+    requires arr1.Length == arr2.Length
+    requires forall i :: 0 <= i < arr1.Length ==> arr1[i] == arr2[i]
+    requires monoid.validMonoid()
+    requires 0 <= l <= arr1.Length && 0 <= r < arr2.Length
+    ensures straightQuery(arr1, l, r, monoid) == straightQuery(arr2, l, r, monoid)
+    decreases r - l
+{
+    if (l > r) {
+        return;
+    }
+    assert arr1[l] == arr2[l];
+    equalArraysEqualQueries(arr1, arr2, l + 1, r, monoid);
+}
+
+lemma equalArraysEqualTrees<T(!new)>(tree: SegmentTree<T>, arr1: array<T>, arr2: array<T>, monoid: Monoid.AbstractMonoid<T>) 
+    requires arr1.Length == arr2.Length
+    requires forall i :: 0 <= i < arr1.Length ==> arr1[i] == arr2[i]
+    requires monoid.validMonoid()
+    requires 0 <= boundaries(tree).0 <= boundaries(tree).1 < arr1.Length
+    requires validTree(tree)
+    requires validTreeValues(tree, arr1, monoid)
+    ensures validTreeValues(tree, arr2, monoid)
+    decreases tree
+{
+    var (l, r) := boundaries(tree);
+    match tree {
+        case Leaf(l, val) => assert arr2[l] == val;
+        case Node(l, m, r, left, right, val) => 
+            equalArraysEqualTrees(left, arr1, arr2, monoid);
+            equalArraysEqualTrees(right, arr1, arr2, monoid);
+            equalArraysEqualQueries(arr1, arr2, l, r, monoid);
+    }
+}
+
+lemma splitSegmentQuery<T(!new)>(arr: array<T>, l: int, m: int, r: int, l1: int, r1: int, monoid: Monoid.AbstractMonoid<T>) 
+    requires monoid.validMonoid()
+    requires 0 <= l <= m <= r < arr.Length
+    requires 0 <= l1 <= r1 < arr.Length
+    ensures straightQuery(arr, maxInt(l, l1), minInt(r, r1), monoid) == 
+        monoid.op(straightQuery(arr, maxInt(l, l1), minInt(m, r1), monoid), straightQuery(arr, maxInt(m + 1, l1), minInt(r, r1), monoid))
+{
+    if m < l1 {
+        assert straightQuery(arr, maxInt(m + 1, l1), minInt(r, r1), monoid) == straightQuery(arr, l1, minInt(r, r1), monoid);
+        assert straightQuery(arr, maxInt(l, l1), minInt(m, r1), monoid) == straightQuery(arr, l1, m, monoid) == monoid.identity();
+        assert straightQuery(arr, l1, minInt(r, r1), monoid) == monoid.op(straightQuery(arr, maxInt(l, l1), minInt(m, r1), monoid), straightQuery(arr, maxInt(m + 1, l1), minInt(r, r1), monoid));
+        assert straightQuery(arr, maxInt(l, l1), minInt(r, r1), monoid) == 
+            monoid.op(straightQuery(arr, maxInt(l, l1), minInt(m, r1), monoid), straightQuery(arr, maxInt(m + 1, l1), minInt(r, r1), monoid));
+        return;
+    }
+    if (m > r1) {
+        assert straightQuery(arr, maxInt(l, l1), minInt(r, r1), monoid) == 
+        monoid.op(straightQuery(arr, maxInt(l, l1), minInt(m, r1), monoid), straightQuery(arr, maxInt(m + 1, l1), minInt(r, r1), monoid));
+        return;
+    }
+    associativeQuery(arr, maxInt(l1, l), m, minInt(r1, r), monoid);
+}
+
+predicate equalStructures<T, U>(tree1: SegmentTree<T>, tree2: SegmentTree<U>) 
+{
+    validTree(tree1) && 
+    validTree(tree2) &&
+    boundaries(tree1) == boundaries(tree2) &&
+    match tree1 {
+        case Node(l1, m1, r1, left1, right1, val1) => match tree2 {
+            case Node(l2, m2, r2, left2, right2, val2) => equalStructures(left1, left2) && equalStructures(right1, right2)
+            case Leaf(_,_) => false
+        }
+        case Leaf(x1, val1) => match tree2 {
+            case Node(_, _, _, _, _, _) => false
+            case Leaf(x2, val2) => x1 == x2
+        }
+    }
+}
+
 class SegmentTreeWrapper<T(!new)>
 {
-    var elems: array<T>
+    var elemsInit: array<T>
+    ghost var elems: array<T>
     var tree: SegmentTree<T>
     var monoid: Monoid.AbstractMonoid<T>
+
+    predicate validStructure() 
+        reads this
+    {
+        elems.Length == elemsInit.Length
+    }
+
+    predicate validSubtree(subTree: SegmentTree<T>)
+        reads this
+        reads elems
+    {
+        monoid.validMonoid() && validTree(subTree) && boundaries(subTree).0 >= 0 && boundaries(subTree).1 < elems.Length && validTreeValues(subTree, elems, monoid)
+    }
+
+    predicate fullTree() 
+        reads this
+    {
+        boundaries(tree) == (0, elems.Length - 1)
+    }
+
+    method buildTreeInner()
+        modifies this
+        requires validStructure()
+        requires monoid.validMonoid()
+        requires elems.Length > 0
+        requires forall i :: 0 <= i < elems.Length ==> elems[i] == elemsInit[i]
+        ensures validSubtree(tree)
+        ensures fullTree()    
+    {
+        var res := buildTree(elemsInit, 0, elemsInit.Length - 1, monoid);
+        tree := res;
+        equalArraysEqualTrees(tree, elemsInit, elems, monoid);
+    }
 
     constructor(arr: array<T>, m: Monoid.AbstractMonoid<T>) 
         requires m.validMonoid()
         requires arr.Length > 0
         ensures monoid.validMonoid()
-        ensures elems.Length == arr.Length
-        ensures validTree(tree)
-        ensures boundaries(tree) == (0, elems.Length - 1)
-        ensures validTreeValues(tree, elems, 0, elems.Length - 1, monoid)
+        ensures elems.Length == arr.Length == elemsInit.Length
     {
         elems := arr;
-        var mon := m;
-        tree := buildTree(arr, 0, arr.Length - 1, mon);
-        monoid := mon;
+        elemsInit := arr;
+        monoid := m;
+        tree := Leaf(0, m.identity());
     }
+
+    function method innerQuery(subTree:SegmentTree<T>, l: int, r: int): (res: T)
+        reads elems
+        reads this
+        requires validSubtree(subTree)
+        requires 0 <= l <= r < elems.Length
+        requires 0 <= boundaries(subTree).0 < elems.Length
+        requires 0 <= boundaries(subTree).1 < elems.Length
+        ensures res == straightQuery(elems, maxInt(boundaries(subTree).0, l), minInt(boundaries(subTree).1, r), monoid)
+        decreases subTree
+    {
+        var (leftPoint, rightPoint) := boundaries(subTree);
+        if (r < leftPoint || l > rightPoint) 
+        then assert monoid.identity() == straightQuery(elems, maxInt(leftPoint, l), minInt(rightPoint, r), monoid); monoid.identity()
+        else if (l <= leftPoint <= rightPoint <= r) 
+            then 
+            assert straightQuery(elems, maxInt(l, leftPoint), minInt(r, rightPoint), monoid) == 
+                straightQuery(elems, leftPoint, rightPoint, monoid);
+            getValue(subTree)
+            else match subTree {
+                case Node(leftPoint, m, rightPoint, left, right, value) =>
+                    splitSegmentQuery(elems, leftPoint, m, rightPoint, l, r, monoid);
+                    assert straightQuery(elems, maxInt(l, leftPoint), minInt(r, rightPoint), monoid) == 
+                        monoid.op(straightQuery(elems, maxInt(leftPoint, l), minInt(m, r), monoid), straightQuery(elems, maxInt(m + 1, l), minInt(rightPoint, r), monoid));
+                    monoid.op(innerQuery(left, l, r), innerQuery(right, l, r))
+                case Leaf(_, val) => assert leftPoint == rightPoint; val
+            }
+    }
+
+    method query(l: int, r: int) returns (res: T)
+        requires 0 <= l < elems.Length
+        requires 0 <= r < elems.Length
+        requires validSubtree(tree)
+        requires fullTree()
+        ensures res == straightQuery(elems, l, r, monoid)
+    {
+        if (l > r) {
+            return monoid.identity();
+        }
+        assert boundaries(tree) == (0, elems.Length - 1);
+        return innerQuery(tree, l, r);
+    }
+    
 }
 
 method Main() {
